non-terminating (?) unit propagation

TheologExercises2026/Exercises/Exercise04.lean
@@ -7,29 +7,142 @@ instance [BEq Atom] (H : HornFormula Atom) : Decidable (H = []) := List.instDeci
 instance [BEq Atom] : BEq (HornClause Atom) where
 beq := fun C1 C2 => C1.head == C2.head && C1.body == C2.body
 
+instance [BEq Atom] [LawfulBEq Atom] : LawfulBEq (HornClause Atom) where
+rfl := by
+  intro C
+  unfold BEq.beq instBEqHornClause
+  simp only [BEq.rfl, Bool.and_self]
+eq_of_beq := by
+  intro C1 C2 beq
+  unfold BEq.beq instBEqHornClause at beq
+  simp at beq
+  rcases beq with ⟨x,y⟩
+
+  sorry
+
 instance [BEq Atom] : BEq (HornFormula Atom) where
 beq := fun H1 H2 => List.beq H1 H2
 
 variable {Atom : Type u}
 
-def Formula.conjunction_from_list : List (Formula Atom) -> Formula Atom
-| .nil => .top
-| .cons hd tl => match tl with
-  | .nil => hd
-  | .cons hd' tl => .and hd (conjunction_from_list (hd'::tl))
+theorem List.removeAll_not_mem [BEq α] [LawfulBEq α] (l : List α) (a : α) (not_mem : a ∉ l) : l.removeAll [a] = l := by
+  unfold removeAll
+  simp only [elem_eq_contains, contains_cons, elem_nil, Bool.or_false, filter_eq_self, Bool.not_eq_eq_eq_not, Bool.not_true]
+  intro b b_mem
+  grind
+
+theorem Formula.disj_from_list_true_iff (L : List (Formula Atom)) (v : Valuation Atom) : v.eval (disjunction_from_list L) ↔ ∃ F, F ∈ L ∧ v.eval F := by
+  induction hL : L generalizing L with
+  | nil =>
+    simp only [List.not_mem_nil, false_and, exists_false, iff_false, Bool.not_eq_true]
+    rfl
+  | cons F L' ih =>
+    simp only [List.mem_cons, exists_eq_or_imp]
+    constructor
+    . intro h
+      cases hF : v.eval F
+      . simp only [Bool.false_eq_true, false_or]
+        have L_eval : v.eval (disjunction_from_list L') := by unfold disjunction_from_list at h; grind
+        exact (ih L' rfl).mp L_eval
+      . apply Or.inl; rfl
+    . intro h
+      rcases h with inl | inr
+      . unfold disjunction_from_list; grind
+      . rcases inr with ⟨G, G_mem, G_eval⟩
+        unfold disjunction_from_list; grind
+
+namespace HornClause
+
+theorem eval_true_iff [BEq Atom] [LawfulBEq Atom] (C : HornClause Atom) (v : Valuation Atom) : v.eval C.toFormula = true ↔ ∃ p, (C.head.isEqSome p ∧ v.eval (.atom p) = true) ∨ (p ∈ C.body ∧ v.eval (.atom p) = false) := by
+  by_cases h : C.head = none ∨ ∃ p, C.head.isEqSome p ∧ !v.eval (Formula.atom p)
+  . constructor
+    . intro eval
+      cases hC : C.head with
+      | none =>
+        simp only [Option.isEqSome_eq_beq_some, Option.none_beq_some, Bool.false_eq_true, false_and, false_or]
+        unfold toFormula at eval
+        simp only [hC, Formula.disj_from_list_true_iff] at eval
+        rcases eval with ⟨l, l_mem, l_eval⟩
+        grind
+      | some p =>
+        simp only [hC, reduceCtorEq, Option.isEqSome_eq_beq_some, Option.some_beq_some, beq_iff_eq,
+          Bool.not_eq_eq_eq_not, Bool.not_true, exists_eq_left', false_or] at h
+        unfold toFormula at eval
+        simp [hC, Formula.disj_from_list_true_iff] at eval
+        rcases eval with inl | inr
+        . grind
+        . rcases inr with ⟨l, l_mem, l_eval⟩
+          grind
+    . intro h_exists
+      rcases h_exists with ⟨p, hp⟩
+      rcases hp with inl | inr
+      . grind
+      . unfold toFormula
+        rcases h with inl' | inr'
+        . simp [inl']
+          have aux : ∃ F, F ∈ List.map (fun a => (Formula.atom a).not) C.body ∧ v.eval F = true := by
+            exists (Formula.atom p).not
+            grind
+          exact (Formula.disj_from_list_true_iff (C.body.map (fun a => (Formula.atom a).not)) v).mpr aux
+        . rcases inr' with ⟨q, q_eq, q_eval⟩
+          simp only [Option.isEqSome_eq_beq_some, beq_iff_eq] at q_eq
+          simp only [q_eq]
+          have aux : ∃ F, F ∈ (Formula.atom q)::(C.body.map (fun a => (Formula.atom a).not)) ∧ v.eval F = true := by
+            exists (Formula.atom p).not
+            grind
+          exact (Formula.disj_from_list_true_iff ((Formula.atom q)::(C.body.map (fun a => (Formula.atom a).not))) v).mpr aux
+  . simp only [Option.isEqSome_eq_beq_some, beq_iff_eq, Bool.not_eq_eq_eq_not, Bool.not_true, not_or, not_exists, not_and, Bool.not_eq_false] at h
+    rcases h with ⟨hd_eq, eval⟩
+    rw [← ne_eq, ← Option.isSome_iff_ne_none, Option.isSome_iff_exists] at hd_eq
+    rcases hd_eq with ⟨p, hd_eq⟩
+    constructor
+    . intro h
+      exists p
+      apply Or.inl
+      grind
+    . intro h
+      unfold toFormula Formula.disjunction_from_list
+      simp only [hd_eq]
+      grind
+
+
+def remove [BEq Atom] (C : HornClause Atom) (p : Atom) : HornClause Atom :=
+mk (if C.head.isEqSome p then none else C.head) (C.body.removeAll [p])
+
+def atoms [BEq Atom] (C : HornClause Atom) : List Atom := match C.head, C.body with
+| none, C' => C'.eraseDups
+| some p, C' => p::C'.eraseDups
+
+def is_unit_clause (C : HornClause Atom) : Bool := match C.head, C.body with
+| none, [_] => true
+| some _, [] => true
+| _, _ => false
+
+def toString [ToString Atom] (C : HornClause Atom) : String := match C.head with
+| none => "{" ++ (C.body.foldl (· ++ "¬" ++ ToString.toString · ++ ", ") "") ++ "}"
+| some p => "{" ++ ToString.toString p ++ ", " ++ C.body.foldl (· ++ "¬" ++ ToString.toString · ++ ", ") "" ++ "}"
+
+instance [ToString S] : ToString (HornClause S) where
+  toString := HornClause.toString
+
+end HornClause
 
 namespace HornFormula
 
 def toFormula (H : HornFormula Atom) : Formula Atom :=
   Formula.list_to_formula (H.map (fun C => C.toFormula))
 
+def atoms [BEq Atom] (H : HornFormula Atom ) : List Atom :=
+  (H.map (fun C => C.atoms)).flatten
+
 theorem eval_toFormula_eq (H : HornFormula Atom) (v : Valuation Atom) : v.eval H.toFormula = (H.map (·.toFormula)).all v.eval := by
   unfold toFormula
   simp
 
 instance : Membership (HornClause Atom) (HornFormula Atom) := List.instMembership
+instance [BEq Atom] [LawfulBEq (HornClause Atom)] {C : HornClause Atom} {H : HornFormula Atom} : Decidable (C ∈ H) := List.instDecidableMemOfLawfulBEq C H
 
-theorem unsat_iff_contains_empty [BEq Atom] (H : HornFormula Atom) : HornClause.empty ∈ H -> H.toFormula.unsatisfiable := by
+theorem unsat_if_contains_empty [BEq Atom] (H : HornFormula Atom) : HornClause.empty ∈ H -> H.toFormula.unsatisfiable := by
   intro empty_mem
   unfold Formula.unsatisfiable
   intro contra
@@ -43,4 +156,108 @@ theorem unsat_iff_contains_empty [BEq Atom] (H : HornFormula Atom) : HornClause.
     have eval_empty : v.eval HornClause.empty.toFormula = true := aux HornClause.empty empty_mem
     contradiction
 
+def unit [BEq Atom] [LawfulBEq (HornClause Atom)] (L : HornClause Atom) (H : HornFormula Atom) : HornFormula Atom :=
+if L ∈ H then match L.head, L.body with
+| none, [p] => (H.filter (fun C => !(C.body.elem p))).map (fun C => C.remove p)
+| some p, [] => (H.filter (fun C => !(C.head.isEqSome p))).map (fun C => C.remove p)
+| _, _ => H
+else H
+
+theorem unit_le [BEq Atom] [LawfulBEq (HornClause Atom)] (L : HornClause Atom) (H : HornFormula Atom) : (H.unit L).length ≤ H.length := by unfold unit; grind
+
+theorem unit_lt [BEq Atom] [ReflBEq Atom] [LawfulBEq Atom] [LawfulBEq (HornClause Atom)] (L : HornClause Atom) (H : HornFormula Atom) : L.is_unit_clause -> L ∈ H -> (H.unit L).length < H.length := by
+  unfold HornClause.is_unit_clause unit
+  simp only [List.elem_eq_contains, Option.isEqSome_eq_beq_some]
+  intro is_unit mem
+  simp only [mem]
+  split at is_unit
+  next p hd_eq b_eq =>
+    have L_eq : L = HornClause.mk none [p] := by rw [← hd_eq, ← b_eq]
+    simp only [if_true, List.length_map, List.length_filter_lt_length_iff_exists]
+    exists HornClause.mk none [p]
+    rw [← L_eq]
+    constructor
+    . exact mem
+    . grind
+  next hd tl p hd_eq tl_eq =>
+    simp only [if_true, List.length_map, List.length_filter_lt_length_iff_exists, Bool.not_eq_eq_eq_not, Bool.not_true, Bool.not_eq_false]
+    exists L
+    constructor
+    . exact mem
+    . grind
+  next x y z => contradiction
+
+theorem sat_iff_unit_sat [BEq Atom] [LawfulBEq Atom] [LawfulBEq (HornClause Atom)] (H : HornFormula Atom) (L : HornClause Atom) : H.toFormula.satisfiable ↔ (H.unit L).toFormula.satisfiable := by
+  unfold Formula.satisfiable
+  constructor
+  . intro sat
+    rcases sat with ⟨v, v_sat⟩
+    exists v
+    unfold unit
+    rw [eval_toFormula_eq] at *
+    by_cases L_mem : L ∈ H
+    . simp only [L_mem, if_true]
+      . split
+        next hd body p hd_eq body_eq =>
+          simp?
+          intro C C_mem
+          by_cases hC : C.body.contains p
+          . apply Or.inl; grind
+          . apply Or.inr
+            have C_eval : v.eval C.toFormula = true := by grind
+            simp at hC
+            rw [HornClause.eval_true_iff] at C_eval
+            have test := (HornClause.eval_true_iff (C.remove p) v).mpr
+            rcases C_eval with ⟨q, hq⟩
+            have aux : ∃ q, (C.remove p).head.isEqSome q = true ∧ v.eval (Formula.atom q) = true ∨ q ∈ (C.remove p).body ∧ v.eval (Formula.atom q) = false := by
+              exists q
+
+              sorry
+
+
+            --rcases C_eval with ⟨q, ⟨q_hd, q_eval⟩ | ⟨q_mem, q_eval⟩⟩
+
+            sorry
+        next hd body p hd_eq body_eq =>
+          simp
+          intro C C_mem
+          by_cases hC : C.head == some p
+          . apply Or.inl; grind
+          . apply Or.inr
+            simp only [Bool.not_eq_true] at hC
+            have C_eval : v.eval C.toFormula = true := by grind
+            unfold HornClause.remove
+            simp only [Option.isEqSome_eq_beq_some, hC, Bool.false_eq_true, ↓reduceIte]
+            by_cases p_mem : p ∈ C.body
+            . have aux' : L.toFormula = (Formula.atom p) := by
+                unfold HornClause.toFormula Formula.disjunction_from_list
+                simp only [hd_eq, body_eq, List.map_nil]
+              have aux : v.eval (Formula.atom p) := by grind
+
+              sorry
+            . have body_eq : C.body.removeAll [p] = C.body := by apply List.removeAll_not_mem; exact p_mem
+              have aux : { head := C.head, body := C.body.removeAll [p] } = C := by rw [body_eq]
+              rw [aux]; exact C_eval
+        . grind
+    . simp only [L_mem, if_false]; grind
+
+  sorry
+
+def unit_clauses : HornFormula Atom -> List (HornClause Atom)
+| [] => []
+| C::H' => if C.is_unit_clause then C::(unit_clauses H') else unit_clauses H'
+
+def unit_propagation [BEq Atom] [LawfulBEq (HornClause Atom)] : HornFormula Atom -> HornFormula Atom
+| [] => []
+| H => match H.unit_clauses with
+  | [] => H
+  | C::_ => unit_propagation (H.unit C)
+
 end HornFormula
+
+
+def K : HornFormula String := [{head := some "b", body := [] : HornClause String}, {head := some "c", body := ["b"] : HornClause String}, {head := some "d", body := ["c"] : HornClause String}, {head := none, body := ["d"] : HornClause String}, {head := some "b", body := ["e"] : HornClause String}]
+def K' : HornFormula String := [{head := some "p", body := [] : HornClause String}, {head := none, body := ["q", "p"] : HornClause String}]
+
+#eval! HornFormula.unit_propagation K'
+#eval! HornFormula.unit_propagation K
